feat(library/init/data): start rbtree module

library/init/data/rbtree/lemmas.lean
@@ -1,51 +1,40 @@
-universes u v
+/-
+Copyright (c) 2017 Microsoft Corporation. All rights reserved.
+Released under Apache 2.0 license as described in the file LICENSE.
+Authors: Leonardo de Moura, Mario Carneiro
+-/
+prelude
+import init.data.rbtree.basic init.meta init.data.nat
 
-inductive rbnode (α : Type u)
-| leaf  {}                                                 : rbnode
-| red_node   (lchild : rbnode) (val : α) (rchild : rbnode) : rbnode
-| black_node (lchild : rbnode) (val : α) (rchild : rbnode) : rbnode
+universes u v
 
 namespace rbnode
 variables {α : Type u} {β : Type v}
 
-@[derive decidable_eq]
-inductive color
-| red | black
-
 open color nat
 
-inductive well_formed : rbnode α → color → nat → Prop
-| leaf_wff       : well_formed leaf black 0
-| red_node_wff   : ∀ {v l r n}, well_formed l black n → well_formed r black n → well_formed (red_node l v r) red n
-| black_node_wff : ∀ {v l r n c₁ c₂}, well_formed l c₁ n → well_formed r c₂ n → well_formed (black_node l v r) black (succ n)
+inductive is_red_black : rbnode α → color → nat → Prop
+| leaf_rb  : is_red_black leaf black 0
+| red_rb   : ∀ {v l r n}, is_red_black l black n → is_red_black r black n → is_red_black (red_node l v r) red n
+| black_rb : ∀ {v l r n c₁ c₂}, is_red_black l c₁ n → is_red_black r c₂ n → is_red_black (black_node l v r) black (succ n)
 
-open well_formed
-
-def fold (f : α → β → β) : rbnode α → β → β
-| leaf b               := b
-| (red_node l v r)   b := fold r (f v (fold l b))
-| (black_node l v r) b := fold r (f v (fold l b))
-
-def rev_fold (f : α → β → β) : rbnode α → β → β
-| leaf b               := b
-| (red_node l v r)   b := rev_fold l (f v (rev_fold r b))
-| (black_node l v r) b := rev_fold l (f v (rev_fold r b))
+open is_red_black
 
 def depth (f : nat → nat → nat) : rbnode α → nat
 | leaf               := 0
 | (red_node l _ r)   := succ (f (depth l) (depth r))
 | (black_node l _ r) := succ (f (depth l) (depth r))
 
-lemma depth_min : ∀ {c n} {t : rbnode α}, well_formed t c n → depth min t ≥ n :=
+lemma depth_min : ∀ {c n} {t : rbnode α}, is_red_black t c n → depth min t ≥ n :=
 begin
   intros c n' t h,
   induction h,
-  case leaf_wff {apply le_refl},
-  case red_node_wff { simp [depth],
+  case leaf_rb {apply le_refl},
+  case red_rb { simp [depth],
     have : min (depth min l) (depth min r) ≥ n,
     { apply le_min, repeat {assumption}},
     apply le_succ_of_le, assumption },
-  case black_node_wff { simp [depth],
+  case black_rb { simp [depth],
     apply succ_le_succ,
     apply le_min, repeat {assumption} }
 end
@@ -58,17 +47,17 @@ private lemma upper_le : ∀ c n, upper c n ≤ 2 * n + 1
 | red n   := by apply le_refl
 | black n := by apply le_succ
 
-lemma depth_max' : ∀ {c n} {t : rbnode α}, well_formed t c n → depth max t ≤ upper c n :=
+lemma depth_max' : ∀ {c n} {t : rbnode α}, is_red_black t c n → depth max t ≤ upper c n :=
 begin
   intros c n' t h,
   induction h,
-  case leaf_wff { simp [max, depth, upper] },
-  case red_node_wff {
+  case leaf_rb { simp [max, depth, upper] },
+  case red_rb {
     suffices : succ (max (depth max l) (depth max r)) ≤ 2 * n + 1,
     { simp [depth, upper, *] at * },
     apply succ_le_succ,
     apply max_le, repeat {assumption}},
-  case black_node_wff {
+  case black_rb {
     have : depth max l ≤ 2*n + 1, from le_trans ih_1 (upper_le _ _),
     have : depth max r ≤ 2*n + 1, from le_trans ih_2 (upper_le _ _),
     suffices new : max (depth max l) (depth max r) + 1 ≤ 2 * n + 2*1,
@@ -77,36 +66,28 @@ begin
   }
 end
 
-lemma depth_max {c n} {t : rbnode α} (h : well_formed t c n) : depth max t ≤ 2 * n + 1:=
+lemma depth_max {c n} {t : rbnode α} (h : is_red_black t c n) : depth max t ≤ 2 * n + 1:=
 le_trans (depth_max' h) (upper_le _ _)
 
-lemma balanced {c n} {t : rbnode α} (h : well_formed t c n) : 2 * depth min t + 1 ≥ depth max t :=
+lemma balanced {c n} {t : rbnode α} (h : is_red_black t c n) : 2 * depth min t + 1 ≥ depth max t :=
 begin
  have : 2 * depth min t + 1 ≥ 2 * n + 1,
  { apply succ_le_succ, apply mul_le_mul_left, apply depth_min h},
  apply le_trans, apply depth_max h, apply this
 end
 
-structure node (α : Type u) :=
-(lchild : rbnode α) (val : α) (rchild : rbnode α)
+lemma balance1_rb {l r t : rbnode α} {y v : α} {c_l c_r c_t n} : is_red_black l c_l n → is_red_black r c_r n → is_red_black t c_t n → ∃ c, is_red_black (balance1 l y r v t) c (succ n) :=
+begin
+  intros h₁ h₂ h₃, cases h₁; cases h₂; repeat {assumption <|> constructor},
+end
 
-def balance1 : rbnode α → α → rbnode α → α → rbnode α → rbnode α
-| (red_node l x r₁) y r₂  v t := red_node (black_node l x r₁) y (black_node r₂ v t)
-| l₁ y (red_node l₂ x r)  v t := red_node (black_node l₁ y l₂) x (black_node r v t)
-| l  y r                  v t := black_node (red_node l y r) v t
-
-lemma balance1_wff {l r t : rbnode α} {y v : α} {c_l c_r c_t n} : well_formed l c_l n → well_formed r c_r n → well_formed t c_t n → ∃ c, well_formed (balance1 l y r v t) c (succ n) :=
+lemma balance2_rb {l r t : rbnode α} {y v : α} {c_l c_r c_t n} : is_red_black l c_l n → is_red_black r c_r n → is_red_black t c_t n → ∃ c, is_red_black (balance2 l y r v t) c (succ n) :=
 begin
   intros h₁ h₂ h₃, cases h₁; cases h₂; repeat {assumption <|> constructor},
 end
 
 lemma balance1_ne_leaf (l : rbnode α) (x r v t) : balance1 l x r v t ≠ leaf :=
 by cases l; cases r; simp [balance1]; intro; contradiction
-
-def balance1_node : rbnode α → α → rbnode α → rbnode α
-| (red_node l x r)   v t := balance1 l x r v t
-| (black_node l x r) v t := balance1 l x r v t
-| leaf               v t := t  /- dummy value -/
 
 lemma balance1_node_ne_leaf {s : rbnode α} (a : α) (t : rbnode α) : s ≠ leaf → balance1_node s a t ≠ leaf :=
 begin
@@ -116,21 +97,6 @@ begin
   case red_node   { simp [balance1_node], apply balance1_ne_leaf },
   case black_node { simp [balance1_node], apply balance1_ne_leaf }
 end
-
-def balance2 : rbnode α → α → rbnode α → α → rbnode α → rbnode α
-| (red_node l x₁ r₁) y r₂  v t := red_node (black_node t v l) x₁ (black_node r₁ y r₂)
-| l₁ y (red_node l₂ x₂ r₂) v t := red_node (black_node t v l₁) y (black_node l₂ x₂ r₂)
-| l  y r                   v t := black_node t v (red_node l y r)
-
-lemma balance2_wff {l r t : rbnode α} {y v : α} {c_l c_r c_t n} : well_formed l c_l n → well_formed r c_r n → well_formed t c_t n → ∃ c, well_formed (balance2 l y r v t) c (succ n) :=
-begin
-  intros h₁ h₂ h₃, cases h₁; cases h₂; repeat {assumption <|> constructor},
-end
-
-def balance2_node : rbnode α → α → rbnode α → rbnode α
-| (red_node l x r)   v t := balance2 l x r v t
-| (black_node l x r) v t := balance2 l x r v t
-| leaf               v t := t /- dummy -/
 
 lemma balance2_ne_leaf (l : rbnode α) (x r v t) : balance2 l x r v t ≠ leaf :=
 by cases l; cases r; simp [balance2]; intro; contradiction
@@ -144,32 +110,8 @@ begin
   case black_node { simp [balance2_node], apply balance2_ne_leaf }
 end
 
-def get_color : rbnode α → color
-| (red_node _ _ _) := red
-| _                := black
-
 section insert
-
 variables (lt : α → α → Prop) [decidable_rel lt]
-
-def ins : rbnode α → α → rbnode α
-| leaf             x  := red_node leaf x leaf
-| (red_node a y b) x  :=
-   match cmp_using lt x y with
-   | ordering.lt := red_node (ins a x) y b
-   | ordering.eq := red_node a x b
-   | ordering.gt := red_node a y (ins b x)
-   end
-| (black_node a y b) x :=
-    match cmp_using lt x y with
-    | ordering.lt :=
-      if a.get_color = red then balance1_node (ins a x) y b
-      else black_node (ins a x) y b
-    | ordering.eq := black_node a x b
-    | ordering.gt :=
-      if b.get_color = red then balance2_node (ins b x) y a
-      else black_node a y (ins b x)
-    end
 
 @[elab_as_eliminator]
 lemma ins.induction_on {p : rbnode α → Prop}
@@ -211,40 +153,7 @@ begin
   }
 end
 
-def insert (t : rbnode α) (x : α) : rbnode α :=
-let r := ins lt t x in
-match r with
-| red_node l v r := black_node l v r
-| _              := r
-end
-
 end insert
-
-section membership
-
-variables (lt : α → α → Prop) [decidable_rel lt]
-
-def contains : rbnode α → α → bool
-| leaf             x := ff
-| (red_node a y b) x :=
-  match cmp_using lt x y with
-  | ordering.lt := contains a x
-  | ordering.eq := tt
-  | ordering.gt := contains b x
-  end
-| (black_node a y b) x :=
-  match cmp_using lt x y with
-  | ordering.lt := contains a x
-  | ordering.eq := tt
-  | ordering.gt := contains b x
-  end
-
-protected def mem : α → rbnode α → Prop
-| a leaf               := false
-| a (red_node l v r)   := mem a l ∨ cmp_using lt a v = ordering.eq  ∨ mem a r
-| a (black_node l v r) := mem a l ∨ cmp_using lt a v = ordering.eq  ∨ mem a r
-
-end membership
 
 end rbnode
 
@@ -338,48 +247,10 @@ end membership_lemmas
 
 end rbnode
 
-open rbnode
-
-meta def rbtree.default_lt : tactic unit :=
-`[apply has_lt.lt]
-
-def rbtree (α : Type u) (lt : α → α → Prop . rbtree.default_lt) [decidable_rel lt] : Type u :=
-{t : rbnode α // true } /- TODO(Leo): add wff condition -/
-
-def mk_rbtree (α : Type u) (lt : α → α → Prop . rbtree.default_lt) [decidable_rel lt] : rbtree α lt :=
-⟨leaf, trivial⟩
-
 namespace rbtree
-variables {α : Type u} {lt : α → α → Prop} {h : decidable_rel lt}
+variables {α : Type u} {lt : α → α → Prop} [decidable_rel lt]
 
-def to_list : @rbtree α lt h → list α
-| ⟨t, _⟩ := t.rev_fold (::) []
-
-def insert : @rbtree α lt h → α → @rbtree α lt h
-| ⟨t, _⟩   x := ⟨t.insert lt x, trivial⟩
-
-def contains : @rbtree α lt h → α → bool
-| ⟨t, _⟩ x := t.contains lt x
-
-protected def mem (a : α) (t : @rbtree α lt h) : Prop :=
-rbnode.mem lt a t.val
-
-instance : has_mem α (@rbtree α lt h) :=
-⟨rbtree.mem⟩
-
-def from_list (l : list α) (lt : α → α → Prop . rbtree.default_lt) [decidable_rel lt] : rbtree α lt :=
-l.foldl insert (mk_rbtree α lt)
-
-lemma mem_insert [is_irrefl α lt] : ∀ (a : α) (t : @rbtree α lt h), a ∈ t.insert a
+lemma mem_insert [is_irrefl α lt] : ∀ (a : α) (t : rbtree α lt), a ∈ t.insert a
 | a ⟨t, _⟩ := t.mem_insert lt a
 
-instance [has_repr α] : has_repr (@rbtree α lt h) :=
-⟨λ t, repr t.to_list⟩
-
 end rbtree
-
-#eval (rbtree.from_list [3, 4, 2, 5, 1] (<)).to_list
-#eval (rbtree.from_list [3, 4, 2, 5, 1] (>)).to_list
-#eval (rbtree.from_list [3, 4, 2, 5]).to_list
-#eval rbtree.from_list [3, 4, 2, 5]
-#eval rbtree.to_list $ rbtree.from_list [3, 4, 2, 5]
