library/init/data/rbtree/basic.lean
@@ -1,0 +1,164 @@
+/-
+Copyright (c) 2017 Microsoft Corporation. All rights reserved.
+Released under Apache 2.0 license as described in the file LICENSE.
+Authors: Leonardo de Moura, Mario Carneiro
+-/
+prelude
+import init.data.ordering
+
+universes u v
+
+inductive rbnode (α : Type u)
+| leaf  {}                                                 : rbnode
+| red_node   (lchild : rbnode) (val : α) (rchild : rbnode) : rbnode
+| black_node (lchild : rbnode) (val : α) (rchild : rbnode) : rbnode
+
+namespace rbnode
+variables {α : Type u} {β : Type v}
+
+inductive color
+| red | black
+
+open color nat
+
+instance color.decidable_eq : decidable_eq color :=
+λ a b, color.cases_on a
+  (color.cases_on b (is_true rfl) (is_false (λ h, color.no_confusion h)))
+  (color.cases_on b (is_false (λ h, color.no_confusion h)) (is_true rfl))
+
+def fold (f : α → β → β) : rbnode α → β → β
+| leaf b               := b
+| (red_node l v r)   b := fold r (f v (fold l b))
+| (black_node l v r) b := fold r (f v (fold l b))
+
+def rev_fold (f : α → β → β) : rbnode α → β → β
+| leaf b               := b
+| (red_node l v r)   b := rev_fold l (f v (rev_fold r b))
+| (black_node l v r) b := rev_fold l (f v (rev_fold r b))
+
+def balance1 : rbnode α → α → rbnode α → α → rbnode α → rbnode α
+| (red_node l x r₁) y r₂  v t := red_node (black_node l x r₁) y (black_node r₂ v t)
+| l₁ y (red_node l₂ x r)  v t := red_node (black_node l₁ y l₂) x (black_node r v t)
+| l  y r                  v t := black_node (red_node l y r) v t
+
+def balance1_node : rbnode α → α → rbnode α → rbnode α
+| (red_node l x r)   v t := balance1 l x r v t
+| (black_node l x r) v t := balance1 l x r v t
+| leaf               v t := t  /- dummy value -/
+
+def balance2 : rbnode α → α → rbnode α → α → rbnode α → rbnode α
+| (red_node l x₁ r₁) y r₂  v t := red_node (black_node t v l) x₁ (black_node r₁ y r₂)
+| l₁ y (red_node l₂ x₂ r₂) v t := red_node (black_node t v l₁) y (black_node l₂ x₂ r₂)
+| l  y r                   v t := black_node t v (red_node l y r)
+
+def balance2_node : rbnode α → α → rbnode α → rbnode α
+| (red_node l x r)   v t := balance2 l x r v t
+| (black_node l x r) v t := balance2 l x r v t
+| leaf               v t := t /- dummy -/
+
+def get_color : rbnode α → color
+| (red_node _ _ _) := red
+| _                := black
+
+section insert
+
+variables (lt : α → α → Prop) [decidable_rel lt]
+
+def ins : rbnode α → α → rbnode α
+| leaf             x  := red_node leaf x leaf
+| (red_node a y b) x  :=
+   match cmp_using lt x y with
+   | ordering.lt := red_node (ins a x) y b
+   | ordering.eq := red_node a x b
+   | ordering.gt := red_node a y (ins b x)
+   end
+| (black_node a y b) x :=
+    match cmp_using lt x y with
+    | ordering.lt :=
+      if a.get_color = red then balance1_node (ins a x) y b
+      else black_node (ins a x) y b
+    | ordering.eq := black_node a x b
+    | ordering.gt :=
+      if b.get_color = red then balance2_node (ins b x) y a
+      else black_node a y (ins b x)
+    end
+
+def insert (t : rbnode α) (x : α) : rbnode α :=
+let r := ins lt t x in
+match r with
+| red_node l v r := black_node l v r
+| _              := r
+end
+
+end insert
+
+section membership
+
+variables (lt : α → α → Prop) [decidable_rel lt]
+
+def contains : rbnode α → α → bool
+| leaf             x := ff
+| (red_node a y b) x :=
+  match cmp_using lt x y with
+  | ordering.lt := contains a x
+  | ordering.eq := tt
+  | ordering.gt := contains b x
+  end
+| (black_node a y b) x :=
+  match cmp_using lt x y with
+  | ordering.lt := contains a x
+  | ordering.eq := tt
+  | ordering.gt := contains b x
+  end
+
+protected def mem : α → rbnode α → Prop
+| a leaf               := false
+| a (red_node l v r)   := mem a l ∨ cmp_using lt a v = ordering.eq  ∨ mem a r
+| a (black_node l v r) := mem a l ∨ cmp_using lt a v = ordering.eq  ∨ mem a r
+
+end membership
+
+inductive well_formed (lt : α → α → Prop) : rbnode α → Prop
+| leaf_wff : well_formed leaf
+| insert_wff {n : rbnode α} (x : α) [decidable_rel lt] : well_formed n → well_formed (insert lt n x)
+
+end rbnode
+
+open rbnode
+
+set_option auto_param.check_exists false
+
+def rbtree (α : Type u) (lt : α → α → Prop . rbtree.default_lt) [decidable_rel lt] : Type u :=
+{t : rbnode α // t.well_formed lt }
+
+def mk_rbtree (α : Type u) (lt : α → α → Prop . rbtree.default_lt) [decidable_rel lt] : rbtree α lt :=
+⟨leaf, well_formed.leaf_wff lt⟩
+
+namespace rbtree
+variables {α : Type u} {lt : α → α → Prop} [decidable_rel lt]
+
+def to_list : rbtree α lt → list α
+| ⟨t, _⟩ := t.rev_fold (::) []
+
+def insert : rbtree α lt → α → rbtree α lt
+| ⟨t, w⟩   x := ⟨t.insert lt x, well_formed.insert_wff x w⟩
+
+def contains : rbtree α lt → α → bool
+| ⟨t, _⟩ x := t.contains lt x
+
+protected def mem (a : α) (t : rbtree α lt) : Prop :=
+rbnode.mem lt a t.val
+
+instance : has_mem α (rbtree α lt) :=
+⟨rbtree.mem⟩
+
+def from_list (l : list α) (lt : α → α → Prop . rbtree.default_lt) [decidable_rel lt] : rbtree α lt :=
+l.foldl insert (mk_rbtree α lt)
+
+instance [has_repr α] : has_repr (rbtree α lt) :=
+⟨λ t, "rbtree_of " ++ repr t.to_list⟩
+
+end rbtree
+
+def rbtree_of {α : Type u} (l : list α) (lt : α → α → Prop . rbtree.default_lt) [decidable_rel lt] : rbtree α lt :=
+rbtree.from_list l lt
