library/init/data/rbtree/default.lean
@@ -1,0 +1,10 @@
+/-
+Copyright (c) 2017 Microsoft Corporation. All rights reserved.
+Released under Apache 2.0 license as described in the file LICENSE.
+Authors: Leonardo de Moura, Mario Carneiro
+-/
+prelude
+import init.data.rbtree.basic init.data.rbtree.lemmas
+
+meta def rbtree.default_lt : tactic unit :=
+`[apply has_lt.lt]
